SStructTT/Static/Progress.lean
@@ -6,39 +6,31 @@ variable {Srt : Type} [inst : SStruct Srt]
 
 inductive Value : Tm Srt -> Prop where
   | srt s i : Value (.srt s i)
-  | pi0 A B s : Value (.pi0 A B s)
-  | pi1 A B s : Value (.pi1 A B s)
-  | lam0 A m s : Value (.lam0 A m s)
-  | lam1 A m s : Value (.lam1 A m s)
-  | sig0 A B s : Value (.sig0 A B s)
-  | sig1 A B s : Value (.sig1 A B s)
-  | tup0 m n s :
+  | pi A B r s : Value (.pi A B r s)
+  | lam A m r s : Value (.lam A m r s)
+  | sig A B r s : Value (.sig A B r s)
+  | tup m n r s :
     Value m ->
-    Value (.tup0 m n s)
-  | tup1 m n s :
-    Value m ->
-    Value n ->
-    Value (.tup1 m n s)
+    (r = .ex -> Value n) ->
+    Value (.tup m n r s)
   | bool : Value .bool
   | tt : Value .tt
   | ff : Value .ff
   | idn A m n : Value (.idn A m n)
   | rfl m : Value (.rfl m)
 
-lemma Typed.pi0_canonical {A B C m : Tm Srt} {s} :
-    [] ⊢ m : C -> C === .pi0 A B s -> Value m ->
-    ∃ A n, m = .lam0 A n s := by
+lemma Typed.pi_canonical {A B C m : Tm Srt} {r s} :
+    [] ⊢ m : C -> C === .pi A B r s -> Value m ->
+    ∃ A n, m = .lam A n r s := by
   generalize e: [] = Γ
   intro ty; induction ty generalizing A B s
   all_goals try (intro eq vl; false_conv)
   case var hs _ => subst_vars; cases hs
-  case lam0 _ A0 B0 m _ _ _ _ _ _ _ =>
-    have ⟨_, _, _⟩ := Conv.pi0_inj eq
+  case lam A0 B0 m _ _ _ _ _ _ _ _ =>
+    have ⟨_, _, _, _⟩ := Conv.pi_inj eq
     subst_vars; exists A0, m
-  case app0 => cases vl
-  case app1 => cases vl
-  case proj0 => cases vl
-  case proj1 => cases vl
+  case app => cases vl
+  case proj => cases vl
   case ite => cases vl
   case rw => cases vl
   case conv ihm _ =>
@@ -48,66 +40,18 @@ lemma Typed.pi0_canonical {A B C m : Tm Srt} {s} :
     . assumption
   all_goals trivial
 
-lemma Typed.pi1_canonical {A B C m : Tm Srt} {s} :
-    [] ⊢ m : C -> C === .pi1 A B s -> Value m ->
-    ∃ A n, m = .lam1 A n s := by
+lemma Typed.sig_canonical {A B C m : Tm Srt} {r s} :
+    [] ⊢ m : C -> C === .sig A B r s -> Value m ->
+    ∃ m1 m2, m = .tup m1 m2 r s := by
   generalize e: [] = Γ
   intro ty; induction ty generalizing A B s
   all_goals try (intro eq vl; false_conv)
   case var hs _ => subst_vars; cases hs
-  case lam1 _ A0 B0 m _ _ _ _ _ _ _ =>
-    have ⟨_, _, _⟩ := Conv.pi1_inj eq
-    subst_vars; exists A0, m
-  case app0 => cases vl
-  case app1 => cases vl
-  case proj0 => cases vl
-  case proj1 => cases vl
-  case ite => cases vl
-  case rw => cases vl
-  case conv ihm _ =>
-    apply ihm
-    . assumption
-    . apply Conv.trans <;> assumption
-    . assumption
-  all_goals trivial
-
-lemma Typed.sig0_canonical {A B C m : Tm Srt} {s} :
-    [] ⊢ m : C -> C === .sig0 A B s -> Value m ->
-    ∃ m1 m2, m = .tup0 m1 m2 s := by
-  generalize e: [] = Γ
-  intro ty; induction ty generalizing A B s
-  all_goals try (intro eq vl; false_conv)
-  case var hs _ => subst_vars; cases hs
-  case app0 => cases vl
-  case app1 => cases vl
-  case tup0 _ A0 B0 m n _ _ _ _ _ _ _ _ =>
-    have ⟨_, _, _⟩ := Conv.sig0_inj eq
+  case app => cases vl
+  case tup A0 B0 m n _ _ _ _ _ _ _ _ _ =>
+    have ⟨_, _, _, _⟩ := Conv.sig_inj eq
     subst_vars; exists m, n
-  case proj0 => cases vl
-  case proj1 => cases vl
-  case ite => cases vl
-  case rw => cases vl
-  case conv ihm _ =>
-    apply ihm
-    . assumption
-    . apply Conv.trans <;> assumption
-    . assumption
-  all_goals trivial
-
-lemma Typed.sig1_canonical {A B C m : Tm Srt} {s} :
-    [] ⊢ m : C -> C === .sig1 A B s -> Value m ->
-    ∃ m1 m2, m = .tup1 m1 m2 s := by
-  generalize e: [] = Γ
-  intro ty; induction ty generalizing A B s
-  all_goals try (intro eq vl; false_conv)
-  case var hs _ => subst_vars; cases hs
-  case app0 => cases vl
-  case app1 => cases vl
-  case tup1 _ A0 B0 m n _ _ _ _ _ _ _ _ =>
-    have ⟨_, _, _⟩ := Conv.sig1_inj eq
-    subst_vars; exists m, n
-  case proj0 => cases vl
-  case proj1 => cases vl
+  case proj => cases vl
   case ite => cases vl
   case rw => cases vl
   case conv ihm _ =>
@@ -123,10 +67,8 @@ lemma Typed.bool_canonical {C m : Tm Srt} :
   intro ty; induction ty
   all_goals try (intro eq vl; false_conv)
   case var hs _ => subst_vars; cases hs
-  case app0 => cases vl
-  case app1 => cases vl
-  case proj0 => cases vl
-  case proj1 => cases vl
+  case app => cases vl
+  case proj => cases vl
   case tt => left; rfl
   case ff => right; rfl
   case ite => cases vl
@@ -144,10 +86,8 @@ lemma Typed.idn_canonical {A C m a b : Tm Srt} :
   intro ty; induction ty
   all_goals try (intro eq vl; false_conv)
   case var hs _ => subst_vars; cases hs
-  case app0 => cases vl
-  case app1 => cases vl
-  case proj0 => cases vl
-  case proj1 => cases vl
+  case app => cases vl
+  case proj => cases vl
   case ite => cases vl
   case rfl m _ _ => exists m
   case rw => cases vl
@@ -165,74 +105,43 @@ theorem Typed.progress {m A : Tm Srt} :
   all_goals try trivial
   case srt => right; constructor
   case var hs _ => subst_vars; cases hs
-  case pi0 => right; constructor
-  case pi1 => right; constructor
-  case lam0 => right; constructor
-  case lam1 => right; constructor
-  case app0 _ n _ tym tyn ihm ihn =>
+  case pi => right; constructor
+  case lam => right; constructor
+  case app _ n r _ tym tyn ihm ihn =>
     subst_vars
     match ihm (Eq.refl _) with
     | .inl ⟨m, _⟩ =>
-      left; exists Tm.app m n
+      left; exists Tm.app m n r
       constructor; assumption
     | .inr vl =>
-      have ⟨A, m, _⟩ := tym.pi0_canonical Conv.R vl
+      have ⟨A, m, _⟩ := tym.pi_canonical Conv.R vl
       subst_vars
       left; exists m.[n/]
       constructor
-  case app1 _ n _ tym tyn ihm ihn =>
+  case sig => right; constructor
+  case tup m n r s _ _ _ _ _ ihm ihn =>
     subst_vars
     match ihm (Eq.refl _) with
     | .inl ⟨m, _⟩ =>
-      left; exists Tm.app m n
-      constructor; assumption
-    | .inr vl =>
-      have ⟨A, m, _⟩ := tym.pi1_canonical Conv.R vl
-      subst_vars
-      left; exists m.[n/]
-      constructor
-  case sig0 => right; constructor
-  case sig1 => right; constructor
-  case tup0 m n s _ _ _ _ _ ihm ihn =>
-    subst_vars
-    match ihm (Eq.refl _) with
-    | .inl ⟨m, _⟩ =>
-      left; exists Tm.tup0 m n s
-      constructor; assumption
-    | .inr vl =>
-      right; constructor; assumption
-  case tup1 m n s _ _ _ _ _ ihm ihn =>
-    subst_vars
-    match ihm (Eq.refl _) with
-    | .inl ⟨m, _⟩ =>
-      left; exists Tm.tup1 m n s
+      left; exists Tm.tup m n r s
       constructor; assumption
     | .inr vl =>
       match ihn (Eq.refl _) with
       | .inl ⟨n, _⟩ =>
-        left; exists Tm.tup1 m n s
+        left; exists Tm.tup m n r s
         constructor; assumption
       | .inr vl =>
-        right; constructor <;> assumption
-  case proj0 C m n _ _ _ _ tym _ _ ihm _ =>
+        right; constructor
+        . assumption
+        . intro; assumption
+  case proj C m n r _ _ _ _ tym _ _ ihm _ =>
     subst_vars
     match ihm (Eq.refl _) with
     | .inl ⟨m, _⟩ =>
-      left; exists Tm.proj C m n
+      left; exists Tm.proj C m n r
       constructor; assumption
     | .inr vl =>
-      have ⟨m1, m2, _⟩ := tym.sig0_canonical Conv.R vl
-      subst_vars
-      left; exists n.[m2,m1/]
-      constructor
-  case proj1 C m n _ _ _ _ tym _ _ ihm _ =>
-    subst_vars
-    match ihm (Eq.refl _) with
-    | .inl ⟨m, _⟩ =>
-      left; exists Tm.proj C m n
-      constructor; assumption
-    | .inr vl =>
-      have ⟨m1, m2, _⟩ := tym.sig1_canonical Conv.R vl
+      have ⟨m1, m2, _⟩ := tym.sig_canonical Conv.R vl
       subst_vars
       left; exists n.[m2,m1/]
       constructor
