SStructTT/Static/Inversion.lean
@@ -4,13 +4,13 @@ open ARS
 namespace Static
 variable {Srt : Type} [inst : SStruct Srt]
 
-lemma Typed.pi0_inv {Γ : Ctx Srt} {A B T s} :
-    Γ ⊢ .pi0 A B s : T ->
+lemma Typed.pi0_inv {Γ : Ctx Srt} {A B T r s} :
+    Γ ⊢ .pi A B r s : T ->
     ∃ sB iB i, A :: Γ ⊢ B : .srt sB iB ∧ T === .srt s i := by
-  generalize e: Tm.pi0 A B s = x
-  intro ty; induction ty generalizing A B s
+  generalize e: Tm.pi A B r s = x
+  intro ty; induction ty generalizing A B r s
   all_goals try trivial
-  case pi0 sB iA iB _ _ _ _ =>
+  case pi sB iA iB _ _ _ _ =>
     cases e; exists sB, iB, (max iA iB); aesop
   case conv eq1 _ _ ih _ =>
     have ⟨sB, iB, i, _, eq2⟩ := ih e
@@ -21,47 +21,13 @@ lemma Typed.pi0_inv {Γ : Ctx Srt} {A B T s} :
       apply Conv.sym eq1
       apply eq2
 
-lemma Typed.pi1_inv {Γ : Ctx Srt} {A B T s} :
-    Γ ⊢ .pi1 A B s : T ->
+lemma Typed.sig_inv {Γ : Ctx Srt} {A B T r s} :
+    Γ ⊢ .sig A B r s : T ->
     ∃ sB iB i, A :: Γ ⊢ B : .srt sB iB ∧ T === .srt s i := by
-  generalize e: Tm.pi1 A B s = x
+  generalize e: Tm.sig A B r s = x
   intro ty; induction ty generalizing A B s
   all_goals try trivial
-  case pi1 sB iA iB _ _ _ _ =>
-    cases e; exists sB, iB, (max iA iB); aesop
-  case conv eq1 _ _ ih _ =>
-    have ⟨sB, iB, i, _, eq2⟩ := ih e
-    exists sB, iB, i
-    constructor
-    . assumption
-    . apply Conv.trans
-      apply Conv.sym eq1
-      apply eq2
-
-lemma Typed.sig0_inv {Γ : Ctx Srt} {A B T s} :
-    Γ ⊢ .sig0 A B s : T ->
-    ∃ sB iB i, A :: Γ ⊢ B : .srt sB iB ∧ T === .srt s i := by
-  generalize e: Tm.sig0 A B s = x
-  intro ty; induction ty generalizing A B s
-  all_goals try trivial
-  case sig0 _ sB iA iB _ _ _ _ _ =>
-    cases e; exists sB, iB, (max iA iB); aesop
-  case conv eq1 _ _ ih _ =>
-    have ⟨sB, iB, i, _, eq2⟩ := ih e
-    exists sB, iB, i
-    constructor
-    . assumption
-    . apply Conv.trans
-      apply Conv.sym eq1
-      apply eq2
-
-lemma Typed.sig1_inv {Γ : Ctx Srt} {A B T s} :
-    Γ ⊢ .sig1 A B s : T ->
-    ∃ sB iB i, A :: Γ ⊢ B : .srt sB iB ∧ T === .srt s i := by
-  generalize e: Tm.sig1 A B s = x
-  intro ty; induction ty generalizing A B s
-  all_goals try trivial
-  case sig1 _ sB iA iB _ _ _ _ _ _ =>
+  case sig sB iA iB _ _ _ _ _ _ =>
     cases e; exists sB, iB, (max iA iB); aesop
   case conv eq1 _ _ ih _ =>
     have ⟨sB, iB, i, _, eq2⟩ := ih e
@@ -92,13 +58,13 @@ lemma Typed.idn_inv {Γ : Ctx Srt} {A T m n} :
       apply Conv.sym eq1
       apply eq2
 
-lemma Typed.lam0_inv' {Γ : Ctx Srt} {A T m s} :
-    Γ ⊢ .lam0 A m s : T ->
-    ∃ B, A :: Γ ⊢ m : B ∧ T === .pi0 A B s := by
-  generalize e: Tm.lam0 A m s = x
-  intro ty; induction ty generalizing A m s
+lemma Typed.lam_inv' {Γ : Ctx Srt} {A T m r s} :
+    Γ ⊢ .lam A m r s : T ->
+    ∃ B, A :: Γ ⊢ m : B ∧ T === .pi A B r s := by
+  generalize e: Tm.lam A m r s = x
+  intro ty; induction ty generalizing A m r s
   all_goals try trivial
-  case lam0 B _ _ _ _ _ _ _ _ =>
+  case lam B _ _ _ _ _ _ _ _ _ =>
     cases e; exists B; aesop
   case conv eq1 _ _ ih _ =>
     have ⟨B, _, eq2⟩ := ih e
@@ -109,48 +75,13 @@ lemma Typed.lam0_inv' {Γ : Ctx Srt} {A T m s} :
       apply Conv.sym eq1
       apply eq2
 
-lemma Typed.lam1_inv' {Γ : Ctx Srt} {A T m s} :
-    Γ ⊢ .lam1 A m s : T ->
-    ∃ B, A :: Γ ⊢ m : B ∧ T === .pi1 A B s := by
-  generalize e: Tm.lam1 A m s = x
-  intro ty; induction ty generalizing A m s
-  all_goals try trivial
-  case lam1 B _ _ _ _ _ _ _ _ =>
-    cases e; exists B; aesop
-  case conv eq1 _ _ ih _ =>
-    have ⟨B, _, eq2⟩ := ih e
-    exists B
-    constructor
-    . assumption
-    . apply Conv.trans
-      apply Conv.sym eq1
-      apply eq2
-
-lemma Typed.tup0_inv' {Γ : Ctx Srt} {T m n s} :
-    Γ ⊢ .tup0 m n s : T ->
-    ∃ A B, Γ ⊢ m : A ∧ Γ ⊢ n : B.[m/] ∧ T === .sig0 A B s := by
-  generalize e: Tm.tup0 m n s = x
+lemma Typed.tup_inv' {Γ : Ctx Srt} {T m n r s} :
+    Γ ⊢ .tup m n r s : T ->
+    ∃ A B, Γ ⊢ m : A ∧ Γ ⊢ n : B.[m/] ∧ T === .sig A B r s := by
+  generalize e: Tm.tup m n r s = x
   intro ty; induction ty generalizing m n s
   all_goals try trivial
-  case tup0 A B _ _ _ _ _ _ _ _ _ _ =>
-    cases e; exists A, B; aesop
-  case conv eq1 _ _ ih _ =>
-    have ⟨A, B, _, _, eq2⟩ := ih e
-    exists A, B
-    and_intros
-    . assumption
-    . assumption
-    . apply Conv.trans
-      apply Conv.sym eq1
-      apply eq2
-
-lemma Typed.tup1_inv' {Γ : Ctx Srt} {T m n s} :
-    Γ ⊢ .tup1 m n s : T ->
-    ∃ A B, Γ ⊢ m : A ∧ Γ ⊢ n : B.[m/] ∧ T === .sig1 A B s := by
-  generalize e: Tm.tup1 m n s = x
-  intro ty; induction ty generalizing m n s
-  all_goals try trivial
-  case tup1 A B _ _ _ _ _ _ _ _ _ _ =>
+  case tup A B _ _ _ _ _ _ _ _ _ _ _ =>
     cases e; exists A, B; aesop
   case conv eq1 _ _ ih _ =>
     have ⟨A, B, _, _, eq2⟩ := ih e
@@ -190,55 +121,29 @@ theorem Typed.validity {Γ : Ctx Srt} {A m} :
   case var wf hs _ =>
     have ⟨s, i, _⟩ := wf.has_typed hs
     exists s, i
-  case pi0 s _ _ iA iB tyA _ _ _ =>
+  case pi s _ _ iA iB tyA _ _ _ =>
     exists s0, (max iA iB + 1)
     constructor
     apply tyA.toWf
-  case pi1 s _ _ iA iB tyA _ _ _ =>
-    exists s0, (max iA iB + 1)
-    constructor
-    apply tyA.toWf
-  case lam0 s _ _ _ tym _ ihm =>
+  case lam s _ _ _ tym _ ihm =>
     have wf := tym.toWf
     cases wf; case cons iA _ _ =>
     have ⟨_, iB, _⟩ := ihm
     exists s, (max iA iB)
     constructor <;> assumption
-  case lam1 s _ _ _ tym _ ihm =>
-    have wf := tym.toWf
-    cases wf; case cons iA _ _ =>
-    have ⟨_, iB, _⟩ := ihm
-    exists s, (max iA iB)
-    constructor <;> assumption
-  case app0 ihm _ =>
+  case app ihm _ =>
     replace ⟨s, i, ihm⟩ := ihm
     have ⟨s, i, j, tyB, eq⟩ := ihm.pi0_inv
     exists s, i
     apply Typed.esubst <;> try first | rfl | assumption
     asimp
-  case app1 ihm _ =>
-    replace ⟨s, i, ihm⟩ := ihm
-    have ⟨s, i, j, tyB, eq⟩ := ihm.pi1_inv
-    exists s, i
-    apply Typed.esubst <;> try first | rfl | assumption
-    asimp
-  case sig0 s _ _ iA iB _ tyA _ _ _ =>
+  case sig iA iB _ _ tyA _ _ _ =>
     exists s0, (max iA iB + 1)
     constructor
     apply tyA.toWf
-  case sig1 s _ _ iA iB _ _ tyA _ _ _ =>
-    exists s0, (max iA iB + 1)
-    constructor
-    apply tyA.toWf
-  case tup0 s i _ _ _ _ _ _ =>
+  case tup s i _ _ _ _ _ _ =>
     exists s, i
-  case tup1 s i _ _ _ _ _ _ =>
-    exists s, i
-  case proj0 s i _ _ _ _ _ _ =>
-    exists s, i
-    apply Typed.esubst <;> try first | rfl | assumption
-    asimp
-  case proj1 s i _ _ _ _ _ _ =>
+  case proj s i _ _ _ _ _ _ =>
     exists s, i
     apply Typed.esubst <;> try first | rfl | assumption
     asimp
@@ -270,12 +175,12 @@ theorem Typed.validity {Γ : Ctx Srt} {A m} :
       apply tya.toWf
   case conv => aesop
 
-lemma Typed.lam0_inv {Γ : Ctx Srt} {A A' B m s s'} :
-    Γ ⊢ .lam0 A m s : .pi0 A' B s' ->
-    A' :: Γ ⊢ m : B ∧ s = s' := by
+lemma Typed.lam_inv {Γ : Ctx Srt} {A A' B m r r' s s'} :
+    Γ ⊢ .lam A m r s : .pi A' B r' s' ->
+    A' :: Γ ⊢ m : B ∧ r = r' ∧ s = s' := by
   intro ty
-  have ⟨B', tym, eq⟩ := ty.lam0_inv'
-  have ⟨_, eqA, eqB⟩ := Conv.pi0_inj eq
+  have ⟨B', tym, eq⟩ := ty.lam_inv'
+  have ⟨_, _, eqA, eqB⟩ := Conv.pi_inj eq
   subst_vars; simp
   have ⟨s, i, tyP⟩ := ty.validity
   have ⟨_, _, _, tyB, _⟩ := tyP.pi0_inv
@@ -285,49 +190,15 @@ lemma Typed.lam0_inv {Γ : Ctx Srt} {A A' B m s s'} :
   apply Typed.conv_ctx eqA tyA'
   apply Typed.conv eqB.sym tym tyB
 
-lemma Typed.lam1_inv {Γ : Ctx Srt} {A A' B m s s'} :
-    Γ ⊢ .lam1 A m s : .pi1 A' B s' ->
-    A' :: Γ ⊢ m : B ∧ s = s' := by
+lemma Typed.tup_inv {Γ : Ctx Srt} {A B m n r r' s s'} :
+    Γ ⊢ .tup m n r s : .sig A B r' s' ->
+    Γ ⊢ m : A ∧ Γ ⊢ n : B.[m/] ∧ r = r' ∧ s = s' := by
   intro ty
-  have ⟨B', tym, eq⟩ := ty.lam1_inv'
-  have ⟨_, eqA, eqB⟩ := Conv.pi1_inj eq
-  subst_vars; simp
-  have ⟨s, i, tyP⟩ := ty.validity
-  have ⟨_, _, _, tyB, _⟩ := tyP.pi1_inv
-  have ⟨_, _, _, tyA'⟩ := tyB.ctx_inv
-  have ⟨_, _, _, tyA⟩ := tym.ctx_inv
-  replace tyB := Typed.conv_ctx eqA.sym tyA tyB
-  apply Typed.conv_ctx eqA tyA'
-  apply Typed.conv eqB.sym tym tyB
-
-lemma Typed.tup0_inv {Γ : Ctx Srt} {A B m n s s'} :
-    Γ ⊢ .tup0 m n s : .sig0 A B s' ->
-    Γ ⊢ m : A ∧ Γ ⊢ n : B.[m/] ∧ s = s' := by
-  intro ty
-  have ⟨A', B', tym, tyn, eq⟩ := ty.tup0_inv'
-  have ⟨_, eqA, eqB⟩ := Conv.sig0_inj eq
+  have ⟨A', B', tym, tyn, eq⟩ := ty.tup_inv'
+  have ⟨_, _, eqA, eqB⟩ := Conv.sig_inj eq
   subst_vars; simp
   have ⟨s, i, tyS⟩ := ty.validity
-  have ⟨_, _, _, tyB, _⟩ := tyS.sig0_inv
-  have ⟨_, _, _, tyA⟩ := tyB.ctx_inv
-  replace tym := Typed.conv eqA.sym tym tyA
-  replace tyB := tyB.subst tym; asimp at tyB
-  constructor
-  . assumption
-  . apply Typed.conv
-    apply Conv.subst _ eqB.sym
-    assumption
-    assumption
-
-lemma Typed.tup1_inv {Γ : Ctx Srt} {A B m n s s'} :
-    Γ ⊢ .tup1 m n s : .sig1 A B s' ->
-    Γ ⊢ m : A ∧ Γ ⊢ n : B.[m/] ∧ s = s' := by
-  intro ty
-  have ⟨A', B', tym, tyn, eq⟩ := ty.tup1_inv'
-  have ⟨_, eqA, eqB⟩ := Conv.sig1_inj eq
-  subst_vars; simp
-  have ⟨s, i, tyS⟩ := ty.validity
-  have ⟨_, _, _, tyB, _⟩ := tyS.sig1_inv
+  have ⟨_, _, _, tyB, _⟩ := tyS.sig_inv
   have ⟨_, _, _, tyA⟩ := tyB.ctx_inv
   replace tym := Typed.conv eqA.sym tym tyA
   replace tyB := tyB.subst tym; asimp at tyB
@@ -350,47 +221,3 @@ lemma Typed.rfl_inv {Γ : Ctx Srt} {A m a b} :
   . apply Typed.conv eqA.sym tym tyA
   . apply eqa.sym
   . apply eqb.sym
-
-lemma Typed.lam0_pi1_false {Γ : Ctx Srt} {A1 A2 B C m s1 s2} :
-    Γ ⊢ .lam0 A1 m s1 : C -> C === .pi1 A2 B s2 -> False := by
-  generalize e: Tm.lam0 A1 m s1 = n
-  intro ty; induction ty generalizing A1 m s1
-  all_goals try trivial
-  case lam0 => intro; false_conv
-  case conv ihm _ =>
-    intro eq; subst_vars
-    apply ihm; rfl
-    apply Conv.trans <;> assumption
-
-lemma Typed.lam1_pi0_false {Γ : Ctx Srt} {A1 A2 B C m s1 s2} :
-    Γ ⊢ .lam1 A1 m s1 : C -> C === .pi0 A2 B s2 -> False := by
-  generalize e: Tm.lam1 A1 m s1 = n
-  intro ty; induction ty generalizing A1 m s1
-  all_goals try trivial
-  case lam1 => intro; false_conv
-  case conv ihm _ =>
-    intro eq; subst_vars
-    apply ihm; rfl
-    apply Conv.trans <;> assumption
-
-lemma Typed.tup0_sig1_false {Γ : Ctx Srt} {A B C m1 m2 s1 s2} :
-    Γ ⊢ .tup0 m1 m2 s1 : C -> C === .sig1 A B s2 -> False := by
-  generalize e: Tm.tup0 m1 m2 s1 = n
-  intro ty; induction ty generalizing m1 m2 s1
-  all_goals try trivial
-  case tup0 => intro; false_conv
-  case conv ihm _ =>
-    intro eq; subst_vars
-    apply ihm; rfl
-    apply Conv.trans <;> assumption
-
-lemma Typed.tup1_sig0_false {Γ : Ctx Srt} {A B C m1 m2 s1 s2} :
-    Γ ⊢ .tup1 m1 m2 s1 : C -> C === .sig0 A B s2 -> False := by
-  generalize e: Tm.tup1 m1 m2 s1 = n
-  intro ty; induction ty generalizing m1 m2 s1
-  all_goals try trivial
-  case tup1 => intro; false_conv
-  case conv ihm _ =>
-    intro eq; subst_vars
-    apply ihm; rfl
-    apply Conv.trans <;> assumption
